Nonogram.lean
@@ -1,2 +1,3 @@
 import Nonogram.Rule
+import Nonogram.LineSolver.Soundness
 import Nonogram.Tactic
